Compiler/Test.v
@@ -1,7 +1,7 @@
-Require Import Kami.AllNotations.
 Require Import Kami.Extraction.
 Require Import BinNat.
 Import FinFun.Fin2Restrict.
+Require Import Kami.AllNotations.
 
 Class toString (X : Type) := {
   to_string : X -> string
@@ -16,7 +16,7 @@ Instance toString_sigma{X}{Y : X -> Type}`{toString X}`{forall x, toString (Y x)
   |}.
 
 Definition cart_prod{X Y}(xs : list X)(ys : list Y) : list (X * Y) :=
-  concat (map (fun x => map (pair x) ys) xs).
+  List.concat (map (fun x => map (pair x) ys) xs).
 
 Inductive FileType :=
   | AsyncF
@@ -393,7 +393,7 @@ Definition make_read : RuleT :=
     Call val : Array num Data <- (read_name tup)($read_index : Bit (Nat.log2_up idxNum));
     Read c : Counter <- "counter";
     LET exp_val : Array num Data <- ITE (#c == $1) $$expected_read_val_second_cycle $$expected_read_val_first_cycle;
-    System ([DispString _  ("rule_" ++ read_name tup ++ ":\n")%string] ++ print_read ($read_index));
+    System ([DispString _  ("rule_" ++ read_name tup ++ ":\n")%string] ++ print_read ($read_index))%list;
     LETA _ : _ <- (print_comparison #val #exp_val);
     Retv
   ).
@@ -408,7 +408,7 @@ Definition make_readReq : RuleT :=
   (("rule_" ++ readReq_name tup)%string,
   fun ty => 
       Call (readReq_name tup)($read_index : Bit (Nat.log2_up idxNum));
-      System ([DispString _  ("rule_" ++ readReq_name tup ++ ":\n")%string] ++ print_read ($read_index));
+      System ([DispString _  ("rule_" ++ readReq_name tup ++ ":\n")%string] ++ print_read ($read_index))%list;
       Retv
   ).
 
